src/proofs/no_slashable_attestations/supporting_lemmas/fnc_invs_1_26.dfy
@@ -2817,54 +2817,54 @@ module Fnc_Invs_1_26
         }
     } 
 
-    lemma lemma_inv26_add_block_to_bn(
+    lemma lemma_inv_consensus_instances_only_for_rcvd_duties_add_block_to_bn(
         s: DVCState,
         block: BeaconBlock,
         s': DVCState 
     )
     requires add_block_to_bn.requires(s, block)
     requires s' == add_block_to_bn(s, block)    
-    requires inv26_body(s)
-    ensures inv26_body(s')
+    requires inv_consensus_instances_only_for_rcvd_duties_body(s)
+    ensures inv_consensus_instances_only_for_rcvd_duties_body(s')
     { }
 
-    lemma lemma_inv26_f_listen_for_attestation_shares(
+    lemma lemma_inv_consensus_instances_only_for_rcvd_duties_f_listen_for_attestation_shares(
         process: DVCState,
         attestation_share: AttestationShare,
         process': DVCState
     )
     requires f_listen_for_attestation_shares.requires(process, attestation_share)
     requires process' == f_listen_for_attestation_shares(process, attestation_share).state        
-    requires inv26_body(process)
-    ensures inv26_body(process')
+    requires inv_consensus_instances_only_for_rcvd_duties_body(process)
+    ensures inv_consensus_instances_only_for_rcvd_duties_body(process')
     { }
 
-    lemma lemma_inv26_f_start_next_duty(process: DVCState, attestation_duty: AttestationDuty, process': DVCState)
+    lemma lemma_inv_consensus_instances_only_for_rcvd_duties_f_start_next_duty(process: DVCState, attestation_duty: AttestationDuty, process': DVCState)
     requires f_start_next_duty.requires(process, attestation_duty)
     requires process' == f_start_next_duty(process, attestation_duty).state   
     requires attestation_duty in process.all_rcvd_duties
-    requires inv26_body(process)
-    ensures inv26_body(process')
+    requires inv_consensus_instances_only_for_rcvd_duties_body(process)
+    ensures inv_consensus_instances_only_for_rcvd_duties_body(process')
     { } 
 
-    lemma lemma_inv26_f_resend_attestation_share(
+    lemma lemma_inv_consensus_instances_only_for_rcvd_duties_f_resend_attestation_share(
         process: DVCState,
         process': DVCState)
     requires f_resend_attestation_share.requires(process)
     requires process' == f_resend_attestation_share(process).state        
-    requires inv26_body(process)
-    ensures inv26_body(process')
+    requires inv_consensus_instances_only_for_rcvd_duties_body(process)
+    ensures inv_consensus_instances_only_for_rcvd_duties_body(process')
     { } 
 
-    lemma lemma_inv26_f_check_for_next_queued_duty(
+    lemma lemma_inv_consensus_instances_only_for_rcvd_duties_f_check_for_next_queued_duty(
         process: DVCState,
         process': DVCState
     )
     requires f_check_for_next_queued_duty.requires(process)
     requires process' == f_check_for_next_queued_duty(process).state    
     requires inv5_body(process)
-    requires inv26_body(process)
-    ensures inv26_body(process')
+    requires inv_consensus_instances_only_for_rcvd_duties_body(process)
+    ensures inv_consensus_instances_only_for_rcvd_duties_body(process')
     decreases process.attestation_duties_queue
     {
         if  && process.attestation_duties_queue != [] 
@@ -2887,16 +2887,16 @@ module Fnc_Invs_1_26
                         )                        
                     );
                     assert inv5_body(process_mod);
-                    lemma_inv26_f_check_for_next_queued_duty(process_mod, process');
+                    lemma_inv_consensus_instances_only_for_rcvd_duties_f_check_for_next_queued_duty(process_mod, process');
                 }
                 else
                 { 
                     var process_mod := process.(
                         attestation_duties_queue := process.attestation_duties_queue[1..]
                     );     
-                    assert inv26_body(process_mod);
+                    assert inv_consensus_instances_only_for_rcvd_duties_body(process_mod);
 
-                    lemma_inv26_f_start_next_duty(process_mod, process.attestation_duties_queue[0], process');
+                    lemma_inv_consensus_instances_only_for_rcvd_duties_f_start_next_duty(process_mod, process.attestation_duties_queue[0], process');
                 }
         }
         else
@@ -2905,7 +2905,7 @@ module Fnc_Invs_1_26
         }
     }
 
-    lemma lemma_inv26_f_att_consensus_decided(
+    lemma lemma_inv_consensus_instances_only_for_rcvd_duties_f_att_consensus_decided(
         process: DVCState,
         id: Slot,
         decided_attestation_data: AttestationData, 
@@ -2914,8 +2914,8 @@ module Fnc_Invs_1_26
     requires f_att_consensus_decided.requires(process, id, decided_attestation_data)
     requires process' == f_att_consensus_decided(process, id, decided_attestation_data).state         
     requires inv5_body(process)
-    requires inv26_body(process)
-    ensures inv26_body(process')
+    requires inv_consensus_instances_only_for_rcvd_duties_body(process)
+    ensures inv_consensus_instances_only_for_rcvd_duties_body(process')
     {
         
         if  || !process.current_attestation_duty.isPresent()
@@ -2949,19 +2949,19 @@ module Fnc_Invs_1_26
             );
 
         assert inv5_body(process);
-        assert inv26_body(process);
+        assert inv_consensus_instances_only_for_rcvd_duties_body(process);
 
         var ret_dvc := f_check_for_next_queued_duty(process).state;
         lemma_inv5_f_check_for_next_queued_duty(process, ret_dvc);
         assert inv5_body(ret_dvc);
         
-        lemma_inv26_f_check_for_next_queued_duty(process, ret_dvc);
-        assert inv26_body(ret_dvc);
+        lemma_inv_consensus_instances_only_for_rcvd_duties_f_check_for_next_queued_duty(process, ret_dvc);
+        assert inv_consensus_instances_only_for_rcvd_duties_body(ret_dvc);
 
         assert process' == ret_dvc;        
     }
 
-    lemma lemma_inv26_f_serve_attestation_duty(
+    lemma lemma_inv_consensus_instances_only_for_rcvd_duties_f_serve_attestation_duty(
         process: DVCState,
         attestation_duty: AttestationDuty,
         process': DVCState
@@ -2969,8 +2969,8 @@ module Fnc_Invs_1_26
     requires f_serve_attestation_duty.requires(process, attestation_duty)
     requires process' == f_serve_attestation_duty(process, attestation_duty).state
     requires inv5_body(process)
-    requires inv26_body(process)
-    ensures inv26_body(process')
+    requires inv_consensus_instances_only_for_rcvd_duties_body(process)
+    ensures inv_consensus_instances_only_for_rcvd_duties_body(process')
     {
         var process_mod := process.(
                 attestation_duties_queue := process.attestation_duties_queue + [attestation_duty],
@@ -2978,12 +2978,12 @@ module Fnc_Invs_1_26
             );        
 
         assert inv5_body(process_mod);
-        assert inv26_body(process_mod);
+        assert inv_consensus_instances_only_for_rcvd_duties_body(process_mod);
         
-        lemma_inv26_f_check_for_next_queued_duty(process_mod, process');        
+        lemma_inv_consensus_instances_only_for_rcvd_duties_f_check_for_next_queued_duty(process_mod, process');        
     }
 
-    lemma lemma_inv26_f_listen_for_new_imported_blocks(
+    lemma lemma_inv_consensus_instances_only_for_rcvd_duties_f_listen_for_new_imported_blocks(
         process: DVCState,
         block: BeaconBlock,
         process': DVCState
@@ -2991,8 +2991,8 @@ module Fnc_Invs_1_26
     requires f_listen_for_new_imported_blocks.requires(process, block)
     requires process' == f_listen_for_new_imported_blocks(process, block).state        
     requires inv5_body(process)
-    requires inv26_body(process)
-    ensures inv26_body(process')
+    requires inv_consensus_instances_only_for_rcvd_duties_body(process)
+    ensures inv_consensus_instances_only_for_rcvd_duties_body(process')
     {
         var new_consensus_instances_already_decided := f_listen_for_new_imported_blocks_helper_1(process, block);
 
@@ -3013,7 +3013,7 @@ module Fnc_Invs_1_26
                 );    
         
         assert inv5_body(process);
-        assert inv26_body(process);
+        assert inv_consensus_instances_only_for_rcvd_duties_body(process);
 
         if process.current_attestation_duty.isPresent() && process.current_attestation_duty.safe_get().slot in att_consensus_instances_already_decided
         {
@@ -3029,13 +3029,13 @@ module Fnc_Invs_1_26
             );
             
             assert inv5_body(process);
-            assert inv26_body(process);
+            assert inv_consensus_instances_only_for_rcvd_duties_body(process);
 
-            lemma_inv26_f_check_for_next_queued_duty(process, process');
+            lemma_inv_consensus_instances_only_for_rcvd_duties_f_check_for_next_queued_duty(process, process');
         }
         else
         {               
-            assert inv26_body(process);
+            assert inv_consensus_instances_only_for_rcvd_duties_body(process);
         }
     } 
 
