src/proofs/no_slashable_attestations/supporting_lemmas/proofs_ind_inv.dfy
@@ -85,7 +85,7 @@ module Proofs_DV_Ind_Inv
         &&  inv22(dv)      
         &&  inv23(dv)  
         &&  inv25(dv)          
-        &&  inv26(dv)  
+        &&  inv_consensus_instances_only_for_rcvd_duties(dv)  
     }
 
     predicate invs_27_37(dv: DVState)       
@@ -201,7 +201,7 @@ module Proofs_DV_Ind_Inv
         lemma_inv22_dv_next(dv, e, dv');                
         // lemma_inv23_dv_next(dv, e, dv');                
         // lemma_inv25_dv_next(dv, e, dv');    
-        // lemma_inv26_dv_next(dv, e, dv');    
+        // lemma_inv_consensus_instances_only_for_rcvd_duties_dv_next(dv, e, dv');    
     }
 
     lemma lemma_ind_inv_dv_next_invs_19_26_helper_2(dv: DVState, e: DV.Event, dv': DVState)       
@@ -210,11 +210,11 @@ module Proofs_DV_Ind_Inv
     requires ind_inv(dv)
     ensures inv23(dv')        
     ensures inv25(dv')
-    ensures inv26(dv')
+    ensures inv_consensus_instances_only_for_rcvd_duties(dv')
     {
         lemma_inv23_dv_next(dv, e, dv');                
         lemma_inv25_dv_next(dv, e, dv');    
-        lemma_inv26_dv_next(dv, e, dv');    
+        lemma_inv_consensus_instances_only_for_rcvd_duties_dv_next(dv, e, dv');    
     }
 
     lemma lemma_ind_inv_dv_next_invs_19_26(dv: DVState, e: DV.Event, dv': DVState)       
